src/Examples/ECC/DownTo.v
@@ -1,0 +1,216 @@
+Require Import Rupicola.Lib.Api.
+
+Section Gallina.
+  Definition downto
+             {state} init count (step:state->nat->state) : state :=
+    fold_left step (rev (seq 0 count)) init.
+End Gallina.
+
+Section Compile.
+  Context {semantics : Semantics.parameters}
+          {semantics_ok : Semantics.parameters_ok semantics}.
+
+  (* in our case, the variables changed are:
+     - P1/P2 pointers
+     - P1/P2 memory values
+     - swap, i (local variables)
+     - s_i (local to each loop instance)
+
+     The parts that need to carry over between iterations are entirely captured
+     in loop state + i; no memory except loop state
+
+     State := fun l '(P1, P2, swap) =>
+                liftexists P1_ptr P2_ptr swap_value,
+                  (emp (map.only_differ locals l
+                                        [swap_var; P1_var; P2_var; si_var]
+                        /\ map.get l swap_var = (if swap
+                                                 then word.of_Z 1
+                                                 else word.of_Z 0)
+                        /\ map.get l P1_var = Some P1_ptr
+                        /\ map.get l P2_var = Some P2_ptr)
+                   * (Point P1_ptr P1 * Point P2_ptr P2))
+
+  *)
+  Local Ltac subst_lets_in_goal :=
+    repeat match goal with
+           | x := _ |- _ =>
+                  lazymatch goal with
+                    |- context [x] => subst x end
+           end.
+
+  Local Ltac handle_downto_locals :=
+    repeat match goal with
+           | H : (?P ?l1 _ * ?R)%sep ?m
+             |- (?P ?l2 _ * ?R)%sep ?m =>
+             replace l2 with l1; [ exact H | ]
+           | H : word.unsigned ?x = _
+             |- context [word.sub ?x (word.of_Z _)] =>
+             rewrite <-(word.of_Z_unsigned x); rewrite H
+           | _ => progress subst_lets_in_goal
+           | _ => progress change 1%Z with (Z.of_nat 1)
+           | _ => rewrite map.get_put_same by auto
+           | _ => rewrite <-word.ring_morph_sub
+           | _ => rewrite <-Nat2Z.inj_sub by lia
+           | _ => reflexivity
+           | _ => solve [eauto]
+           end.
+
+  Local Ltac use_cmd_hyp :=
+    let H := lazymatch goal with
+             | H: context [WeakestPrecondition.cmd _ ?impl]
+               |- WeakestPrecondition.cmd _ ?impl _ _ _ _ => H end in
+    eapply Proper_cmd;
+    [ solve [apply Proper_call]
+    | repeat intro | eapply H ].
+
+  (* TODO: move *)
+  Lemma skipn_seq_step n start len :
+    skipn n (seq start len) = seq (start + n) (len - n).
+  Admitted. (* TODO *)
+
+  (* TODO: move *)
+  Lemma fold_left_skipn_seq {A} i count (step :A -> _) init :
+    0 < i <= count ->
+    step (fold_left step (rev (skipn i (seq 0 count))) init) (i-1) =
+    fold_left step (rev (skipn (i-1) (seq 0 count))) init.
+  Proof.
+    intros. rewrite !skipn_seq_step, !Nat.add_0_l.
+    replace (count - (i - 1)) with (S (count - i)) by lia.
+    cbn [seq rev]. rewrite fold_left_app. cbn [fold_left].
+    replace (S (i-1)) with i by lia.
+    reflexivity.
+  Qed.
+
+  Lemma compile_downto :
+    forall (locals: Semantics.locals) (mem: Semantics.mem)
+      tr R R' functions T (pred: T -> _ -> Prop)
+      {state} (init : state) count wcount step step_impl k k_impl i_var
+      (State : Semantics.locals -> state -> Semantics.mem -> Prop),
+      (State (map.put locals i_var wcount) init * R')%sep mem ->
+      word.unsigned wcount = Z.of_nat count ->
+      0 < count ->
+      let v := downto init count step in
+      (let head := v in
+       (* loop iteration case *)
+       forall tr l li m st i,
+         let wi := word.of_Z (Z.of_nat i) in
+         (State l st * R')%sep m ->
+         li = map.put l i_var wi ->
+         WeakestPrecondition.cmd
+           (WeakestPrecondition.call functions) step_impl tr m li
+           (fun tr' m' l' =>
+              tr = tr'
+              /\ map.get l' i_var = Some wi (* didn't change i *)
+              /\ (State l' (step st i) * R')%sep m')) ->
+      (let head := v in
+       (* post-loop case *)
+       forall tr l m,
+         (State l head * R')%sep m ->
+         WeakestPrecondition.cmd
+           (WeakestPrecondition.call functions) k_impl tr m l
+           (fun tr' m' l' =>
+              tr = tr' /\ (pred (k head) * R)%sep m')) ->
+      (let head := v in
+       (* while (i = n; 0 < i; pass)
+          { i--; step i } *)
+       find (cmd.seq
+               (cmd.seq
+                  (cmd.set i_var (expr.literal (Z.of_nat count)))
+                  (cmd.while
+                     (expr.op bopname.ltu
+                              (expr.literal 0) (expr.var i_var))
+                     (cmd.seq
+                        (cmd.set i_var
+                                 (expr.op bopname.sub
+                                          (expr.var i_var)
+                                          (expr.literal 1)))
+                        step_impl)))
+               k_impl)
+       implementing (pred (dlet head k))
+       with-locals locals and-memory mem and-trace tr and-rest R
+       and-functions functions).
+  Proof.
+    repeat straightline'.
+
+    (* handle while *)
+    WeakestPrecondition.unfold1_cmd_goal;
+      (cbv beta match delta [WeakestPrecondition.cmd_body]).
+    exists nat, lt.
+    exists (fun i t m l =>
+              let st :=
+                  fold_left step (rev (skipn i (seq 0 count))) init in
+              (State l st * R')%sep m
+              /\ i <= count
+              /\ tr = t
+              /\ (exists wi,
+                     word.unsigned wi = Z.of_nat i
+                     /\ map.get l i_var = Some wi)).
+    ssplit; eauto using lt_wf; [ | ].
+
+    { cbv zeta.
+      exists count; ssplit; [ | | | exists wcount];
+        repeat match goal with
+               | H : _ = Z.of_nat count |- _ => rewrite <-H
+               | _ => rewrite map.put_put_same by auto
+               | _ => rewrite map.get_put_same by auto
+               | _ => rewrite word.of_Z_unsigned
+               | _ => rewrite skipn_all2 by (rewrite seq_length; lia)
+               | _ => progress subst_lets_in_goal
+               | _ => progress cbn [rev]
+               | _ => solve [eauto]
+               end. }
+
+    { intros. cleanup.
+      repeat straightline'.
+      lazymatch goal with x := context [word.ltu] |- _ => subst x end.
+      rewrite word.unsigned_ltu, word.unsigned_of_Z_0.
+      match goal with
+      | H1 : ?y = Z.of_nat ?x, H2 : 0 < ?x |- _ =>
+        assert (0 < y)%Z by
+            (rewrite H1; change 0%Z with (Z.of_nat 0);
+             apply Nat2Z.inj_lt; auto)
+      end.
+      destruct_one_match;
+        rewrite ?word.unsigned_of_Z_0, ?word.unsigned_of_Z_1;
+        ssplit; try lia; [ | ].
+      { repeat straightline'.
+        use_cmd_hyp; [ | solve [handle_downto_locals] .. ].
+        cleanup; subst.
+        lazymatch goal with
+        | H : word.unsigned ?w = Z.of_nat ?x
+          |- exists i : nat, _ /\ i < ?x =>
+          exists (x-1)%nat; ssplit;
+            lazymatch goal with
+            | |- exists _, _ => exists (word.sub w (word.of_Z 1))
+            | |- sep _ _ _ =>
+              rewrite <-fold_left_skipn_seq by lia; assumption
+            | _ => auto; try lia
+            end
+        end; [ ].
+        ssplit; handle_downto_locals; [ ].
+        rewrite word.unsigned_of_Z.
+        lazymatch goal with
+        | H : word.unsigned ?w = Z.of_nat ?i
+          |- word.wrap (Z.of_nat (?i - 1)) = Z.of_nat (?i - 1) =>
+          pose proof (word.unsigned_range w);
+            apply Z.mod_small; rewrite Nat2Z.inj_sub, <-H by lia
+        end.
+        lia. }
+      { repeat straightline'.
+        match goal with
+        | H : (word.unsigned ?x <= 0)%Z |- _ =>
+          let H' := fresh in
+          assert (word.unsigned x = 0%Z) as H'
+              by (pose proof word.unsigned_range x; lia)
+        end.
+        match goal with
+        | H : context [skipn ?i] |- _ =>
+          replace i with 0 in H by lia; cbn [skipn] in H
+        end.
+        use_cmd_hyp.
+        { cbv [postcondition_norets postcondition_for].
+          cleanup. ssplit; auto. }
+        { subst_lets_in_goal. assumption. } } }
+  Qed.
+
+End Compile.
